proof/correctness/MLKEM_keccak_ref.ec
@@ -1,0 +1,133 @@
+require import AllCore IntDiv List.
+require export FIPS202_Keccakf1600 FIPS202_SHA3_Spec.
+require export Keccak1600_Spec Keccakf1600_Spec.
+
+
+(***THESE ASSUMPTIONS MAP SHA OPERATORS FROM SPEC TO CODE IN
+    THE IMPLEMENTATION ****)
+
+require import Symmetric MLKEMFCLib.
+from Jasmin require import JModel.
+
+require import Array1152 Array960 Array128 Array64 Array34 Array33 Array32.
+
+require import Jkem.
+
+axiom sha3_512_33_64 seed : 
+   phoare [Jkem.M(Jkem.Syscall)._sha3512_33 : 
+               arg.`2 = seed ==>
+               Array32.init(fun i => res.[i]) = (SHA3_512_33_64 seed).`1 /\
+               Array32.init(fun i => res.[32 + i]) = (SHA3_512_33_64 seed).`2  ] = 1%r.
+
+axiom shake_absorb (seed : W8.t Array34.t): 
+   phoare [Jkem.M(Jkem.Syscall)._shake128_absorb34 : 
+               arg.`2 = seed ==>
+               res = SHAKE128_ABSORB_34 
+                         (Array32.init (fun k => seed.[k])) (seed.[32]) (seed.[33]) ] = 1%r.
+
+axiom shake_squeeze state : 
+   phoare [Jkem.M(Jkem.Syscall)._shake128_squeezeblock : 
+               arg.`1 = state ==>
+               res = SHAKE128_SQUEEZE_168 state ] = 1%r.
+
+axiom shake256_33_128 seed : 
+   phoare [Jkem.M(Jkem.Syscall)._shake256_128_33 : 
+               arg.`2 = seed ==>
+               res = SHAKE256_33_128 (Array32.init (fun i => seed.[i])) seed.[32] ] = 1%r.
+
+
+axiom shake256_33_128_ll: islossless M(Syscall)._shake256_128_33.
+
+
+
+axiom pkH_sha mem _ptr: 
+    phoare [Jkem.M(Jkem.Syscall)._isha3_256 :
+          arg.`2 = W64.of_int _ptr /\
+          arg.`3 = W64.of_int (3*384+32) /\
+          valid_ptr _ptr 1184 /\
+          Glob.mem = mem
+          ==> 
+          Glob.mem = mem /\
+          res = SHA3_256_1184_32
+            (Array1152.init (fun k =>  mem.[_ptr+k]),
+            (Array32.init (fun k => mem.[_ptr+1152+k])))] = 1%r.
+
+axiom j_shake mem _pout _pin1 _pin2: 
+    phoare [Jkem.M(Syscall)._shake256_1120_32  :
+          arg = (W64.of_int _pout,W64.of_int _pin1,W64.of_int _pin2) /\
+          valid_ptr _pout 32 /\
+          valid_ptr _pin1 32 /\
+          valid_ptr _pin2 1088 /\
+          Glob.mem = mem
+          ==> 
+          touches Glob.mem mem _pout 32 /\
+          (Array32.init (fun k =>  Glob.mem.[_pout+k])) = 
+             SHAKE_256_1120_32 (Array32.init (fun k => mem.[_pin1+k])) 
+                            (Array960.init (fun k => mem.[_pin2+k]), Array128.init (fun k => mem.[_pin2+960+k])) ] = 1%r.
+
+axiom sha_g buf: 
+    phoare [Jkem.M(Jkem.Syscall)._sha3_512_64 :
+          arg.`2 = buf
+          ==> 
+          let bytes = SHA3_512_64_64 (Array32.init (fun k => buf.[k])) 
+                                     (Array32.init (fun k => buf.[k+32])) in
+          res = Array64.init (fun k => if k < 32 then bytes.`1.[k] else bytes.`2.[k-32])] = 1%r.
+
+
+(*
+axiom sha3_512_33_64 buf seed : 
+   phoare [Jkem.M(Jkem.Syscall)._sha3512_33 : 
+               arg = (buf,seed) ==>
+               Array32.init(fun i => res.[i]) = (SHA3_512_33_64 seed).`1 /\
+               Array32.init(fun i => res.[32 + i]) = (SHA3_512_33_64 seed).`2  ] = 1%r.
+
+axiom shake_absorb (seed : W8.t Array34.t) state : 
+   phoare [Jkem.M(Jkem.Syscall)._shake128_absorb34 : 
+               arg = (state,seed) ==>
+               res = SHAKE128_ABSORB_34 
+                         (Array32.init (fun k => seed.[k])) (seed.[32]) (seed.[33]) ] = 1%r.
+
+axiom shake_squeeze buf state : 
+   phoare [Jkem.M(Jkem.Syscall)._shake128_squeezeblock : 
+               arg = (state,buf) ==>
+               res = SHAKE128_SQUEEZE_168 state ] = 1%r.
+
+axiom shake256_33_128 buf seed : 
+   phoare [Jkem.M(Jkem.Syscall)._shake256_128_33 : 
+               arg = (buf,seed) ==>
+               res = SHAKE256_33_128 (Array32.init (fun i => seed.[i])) seed.[32] ] = 1%r.
+
+
+axiom pkH_sha mem _ptr inp: 
+    phoare [Jkem.M(Jkem.Syscall)._isha3_256 :
+          arg = (inp,W64.of_int _ptr,W64.of_int (3*384+32)) /\
+          valid_ptr _ptr 1184 /\
+          Glob.mem = mem
+          ==> 
+          Glob.mem = mem /\
+          res = SHA3_256_1184_32
+            (Array1152.init (fun k =>  mem.[_ptr+k]),
+            (Array32.init (fun k => mem.[_ptr+1152+k])))] = 1%r.
+
+axiom j_shake mem _pout _pin1 _pin2: 
+    phoare [Jkem.M(Syscall)._shake256_1120_32  :
+          arg = (W64.of_int _pout,W64.of_int _pin1,W64.of_int _pin2) /\
+          valid_ptr _pout 32 /\
+          valid_ptr _pin1 32 /\
+          valid_ptr _pin2 1088 /\
+          Glob.mem = mem
+          ==> 
+          touches Glob.mem mem _pout 32 /\
+          (Array32.init (fun k =>  Glob.mem.[_pout+k])) = 
+             SHAKE_256_1120_32 (Array32.init (fun k => mem.[_pin1+k])) 
+                            (Array960.init (fun k => mem.[_pin2+k]), Array128.init (fun k => mem.[_pin2+960+k])) ] = 1%r.
+
+axiom sha_g buf inp: 
+    phoare [Jkem.M(Jkem.Syscall)._sha3_512_64 :
+          arg = (inp,buf)
+          ==> 
+          let bytes = SHA3_512_64_64 (Array32.init (fun k => buf.[k])) 
+                                     (Array32.init (fun k => buf.[k+32])) in
+          res = Array64.init (fun k => if k < 32 then bytes.`1.[k] else bytes.`2.[k-32])] = 1%r.
+
+*)
